working on induction scheme

verif/GlobalExtends.v
@@ -16,11 +16,61 @@ Require Import Values.
 Require Import Eager.
 Require Import Bitstream.
 Require Import Lib.
+Require Import EagerEvalInd.
+
+Definition global_extends (ge ge' : genv) : Prop :=
+  forall id v,
+    ge id = Some v ->
+    ge' id = Some v.
+
+
+Lemma global_extends_refl :
+  forall GE,
+    global_extends GE GE.
+Proof.
+  intros.
+  unfold global_extends. auto.
+Qed.
 
 
 Definition name_irrel {A : Type} (E : ident -> option A) : Prop :=
   forall id id',
     if ident_eq id id' then E id = E id' else True.
+
+Lemma global_extends_extend_r :
+  forall ge ge',
+    global_extends ge ge' ->
+    name_irrel ge ->
+    forall id exp,
+      ge id = None ->
+      global_extends ge (extend ge' id exp).
+Proof.
+  intros.
+  unfold global_extends in *.
+  intros.
+  unfold extend. unfold name_irrel in *.
+  specialize (H0 id0 id).
+  destruct (ident_eq id0 id).
+  congruence. eapply H; eauto.
+Qed.
+
+Lemma global_extends_eager_eval :
+    forall expr v ge TE SE,
+      eager_eval_expr ge TE SE expr v ->
+      forall GE,
+        global_extends ge GE ->
+        eager_eval_expr GE TE SE expr v.
+Proof.
+  (*   induction 1 using eager_eval_expr_useful; intros. *)
+Admitted.
+
+(* lowercase is concrete, uppercase is abstract *)
+(* wf_env lets this proof be used over a variety of environments that meet the proper constraints *)
+Definition wf_env (ge GE : genv) (TE : tenv) (SE : senv)  : Prop :=
+  name_irrel ge /\ name_irrel GE /\ name_irrel TE /\ name_irrel SE /\ (*finite GE /\*)
+  (forall id,
+      ge id <> None -> (TE id = None /\ SE id = None /\ ge id = GE id)).
+
 
 Lemma name_irrel_diff_results :
   forall {A} E id id',
@@ -37,126 +87,6 @@ Proof.
   exists n. eauto.
 Qed.
 
-Definition same_values (ge GE : genv) : Prop :=
-  forall id v,
-    ge id = Some v ->
-    GE id = Some v.
-
-Definition finite (ge : genv) : Prop :=
-  exists l,
-  forall id,
-    ge id <> None <-> In id l.
-
-Fixpoint make_ge (l : list (ident * Expr)) (ge : genv) : genv :=
-  match l with
-  | nil => ge
-  | (id,exp) :: l' =>
-    let ge' := make_ge l' ge in
-    extend ge' id exp
-  end.
-
-Definition finite' (ge : genv) (l : list (ident * Expr)) : Prop :=
-  forall id,
-    ge id = make_ge l gempty id.
-
-Fixpoint id_In (ide : (ident * Expr)) (l : list (ident * Expr)) : Prop :=
-  match l with
-  | nil => False
-  | (id,e) :: l =>
-    match ide with
-    | (id',e') => (fst id = fst id' /\ e = e') \/ id_In (id',e') l
-    end
-  end.
-
-(* lowercase is concrete, uppercase is abstract *)
-(* wf_env lets this proof be used over a variety of environments that meet the proper constraints *)
-Definition wf_env (ge GE : genv) (TE : tenv) (SE : senv)  : Prop :=
-  name_irrel ge /\ name_irrel GE /\ name_irrel TE /\ name_irrel SE /\ (*finite GE /\*)
-  (forall id,
-      ge id <> None -> (TE id = None /\ SE id = None /\ ge id = GE id)).
-
-Definition global_extends (ge GE : genv) : Prop :=
-  same_values ge GE /\
-  finite ge /\ finite GE /\
-  name_irrel ge.
-
-(* TODO *)
-(*
-Definition global_extends (ge GE : genv) : Prop :=
-  (forall id v,
-    ge id = Some v ->
-    GE id = Some v) /\
-(*  (forall TE SE expr v,
-      eager_eval_expr ge TE SE expr v ->
-      eager_eval_expr GE TE SE expr v) /\*)
-  exists l, (forall id x, ge id = Some x -> In x l) /\
-              exists l',
-                (forall id x, GE id = Some x -> In x l') /\
-                (forall x, In x l -> In x l').
-                                           
-*)
-
-Lemma global_extends_refl :
-  forall ge GE TE SE,
-    wf_env ge GE TE SE ->
-    global_extends GE GE.
-Proof.
-  intros.
-  unfold wf_env in *.
-  repeat match goal with
-         | [ H : _ /\ _ |- _ ] => destruct H
-         end.
-  unfold global_extends. split; auto.
-  unfold same_values.
-  intros. auto.
-Admitted.
-
-Lemma global_extends_extend_r :
-  forall ge ge',
-    global_extends ge ge' ->
-    forall id exp,
-      ge id = None ->
-      global_extends ge (extend ge' id exp).
-Proof.
-  intros.
-  unfold global_extends in *.
-  repeat match goal with
-         | [ H : _ /\ _ |- _ ] => destruct H
-         end.
-  split; auto; [idtac | split; auto].
-  unfold same_values in *.
-  intros.
-  destruct (ident_eq id0 id) eqn:?; auto.
-  unfold name_irrel in *. 
-  specialize (H3 id0 id). rewrite Heqs in H3.
-  congruence.
-  unfold extend.
-  rewrite Heqs.
-  eapply H; eauto.
-  split; auto.
-  
-  admit. (* finite extends to finite *)
-  
-Admitted.
-
-(*
-Inductive eager_eval_expr_listenv (ge : list (ident * Expr)) : tenv -> senv -> Expr -> strictval -> Prop :=
-| eval_bind_list :
-    forall TE SE e v,
-      eager_eval_expr (make_ge ge gempty) TE SE e v ->
-      eager_eval_expr_listenv ge TE SE e v.
-
-Lemma eval_with_list_same :
-  forall ge TE SE e v,
-    eager_eval_expr (make_ge ge gempty) TE SE e v <->
-    eager_eval_expr_listenv ge TE SE e v.
-Proof.
-  intros; split.
-  intros. econstructor; eauto.
-  intros.
-  inversion H. eauto.
-Qed.
- *)
 
 Lemma name_irrel_extend :
   forall {A} E id (x : A),
@@ -190,300 +120,3 @@ Proof.
     auto; congruence.
 Qed.
 
-
-Lemma finite'_id_In :
-  forall l ge id exp,
-    ge id = Some exp ->
-    finite' ge l ->
-    id_In (id,exp) l.
-Proof.
-  induction l; intros;
-    unfold finite' in H0;
-    erewrite H0 in H. simpl in H. unfold gempty in *.  congruence.
-  simpl in H. destruct a.
-  unfold extend in H.
-  destruct (ident_eq id i). simpl. left. split; congruence.
-  simpl. right. eapply IHl; eauto.
-  unfold finite'. intros. reflexivity.
-Qed.
-
-
-Lemma make_ge_id_in :
-  forall l id exp,
-    make_ge l gempty id = Some exp ->
-    id_In (id,exp) l.
-Proof.
-  induction l; intros.
-  simpl in H. unfold gempty in H. congruence.
-  simpl in H. destruct a.
-  unfold extend in H. destruct (ident_eq id i).
-  simpl. left. split; congruence.
-  simpl. right.
-  eapply IHl; eauto.
-Qed.
-
-Lemma free_ge :
-  forall expr ge TE SE v,  
-    eager_eval_expr ge TE SE expr v ->
-    forall ge',
-      (forall id e, ge id = Some e ->
-                    ge' id = Some e /\
-                    forall TE SE v,
-                      eager_eval_expr ge TE SE e v ->
-                      eager_eval_expr ge' TE SE e v
-      ) ->
-      eager_eval_expr ge' TE SE expr v.
-Proof.
-  intro.
-  eapply Expr_ind_useful with (e := expr); intros.
-  Focus 8.
-  inversion H. subst.
-  econstructor; eauto.
-  subst.
-  eapply H0 in H3. destruct H3.
-  eapply H3 in H6. eapply eager_eval_global_var; eauto.
-
-  inversion H0. subst.
-  econstructor; eauto.
-  admit. admit.
-
-  inversion H0. subst.
-  econstructor; eauto.
-  unfold Pl in H.
-  eapply Forall_Forall2_implies; try eassumption.
-  intros. simpl in H2.
-  eapply H2; eauto.
-
-  (* This is true, can finish proof if needed *)
-Admitted.
-
-
-
-Lemma eager_eval_expr_from_make_ge :
-  forall expr l ge TE SE v,
-    finite' ge l ->
-    (forall id exp',
-        id_In (id,exp') l ->
-        forall v',
-          eager_eval_expr (make_ge l gempty) TE SE exp' v' ->
-          eager_eval_expr ge TE SE exp' v') ->
-    eager_eval_expr (make_ge l gempty) TE SE expr v ->
-    eager_eval_expr ge TE SE expr v.
-Proof.
-  intro.
-  eapply Expr_ind_useful with (e := expr); intros;
-    try solve [
-           try (match goal with
-                 | [ H : eager_eval_expr _ _ _ _ _ |- _ ] => inversion H; clear H
-                 end);
-          econstructor; eauto].
-  Focus 7.
-  inversion H1. subst.
-  econstructor; eauto.
-  subst. eapply eager_eval_global_var; eauto.
-  unfold finite' in *. rewrite H. eauto.
-  eapply H0; eauto.
-  eapply finite'_id_In.
-  unfold finite' in H. rewrite <- H in H4.
-  eassumption. eauto.
-
-  inversion H2. subst. econstructor; eauto.
-  (* this is provable *)
-
-  
-Admitted.
-
-
-Lemma eager_eval_expr_make_ge :
-  forall expr l ge TE SE v,
-    finite' ge l ->
-    (forall id exp',
-        id_In (id,exp') l ->
-        forall v',
-          eager_eval_expr ge TE SE exp' v' ->
-          eager_eval_expr (make_ge l gempty) TE SE exp' v') ->
-    eager_eval_expr ge TE SE expr v ->
-    eager_eval_expr (make_ge l gempty) TE SE expr v.
-Proof.
-  intro.
-  eapply Expr_ind_useful with (e := expr); intros.
-
-  unfold Pl in *. inversion H2; subst; econstructor; eauto.
-  admit. admit.
-
-  admit. admit. admit. admit.
-  admit. admit. 
-
-  subst. inversion H1; try solve [econstructor; eauto]. subst. eapply eager_eval_global_var; eauto.
-  unfold finite' in *. rewrite H in H4. eauto.
-  eapply H0; eauto.
-  instantiate (1 := id).
-  eapply finite'_id_In; eauto.
-
-  admit. admit. admit.
-  admit. admit. admit.
-
-  (* This one's true, will take a while to prove *)  
-Admitted.
-
-
-(* at the end of the day I need this fact *)
-Lemma global_extends_eager_eval :
-    forall expr v ge TE SE,
-      eager_eval_expr ge TE SE expr v ->
-      forall GE,
-        global_extends ge GE ->
-        eager_eval_expr GE TE SE expr v.
-Proof.
-  intros.
-  unfold global_extends in *.
-  repeat match goal with
-         | [ H : _ /\ _ |- _ ] => destruct H
-         end.
-  unfold finite in *.
-  destruct H1 as [l]. destruct H2 as [l'].
-  unfold same_values in *.
-  assert (forall id, In id l -> In id l').
-  intros. eapply H2.
-  destruct (ge id) eqn:?.
-  eapply H0 in Heqo. congruence.
-  erewrite <- H1 in H4. congruence.
-  
-  
-  
-Admitted.
-
-
-
-(*
-(* is this necessary? *)
-Lemma finite_make_ge :
-  forall ge,
-    finite ge ->
-    name_irrel ge ->
-    exists l,
-      forall id,
-        ge id  = make_ge l gempty id.
-Proof.
-  intros. unfold finite in *.
-  destruct H.
-  generalize dependent ge.
-  induction x; intros. exists nil.
-  simpl in H. intros.
-  destruct (ge id) eqn:?.
-  assert (ge id <> None) by congruence.
-  erewrite H in H1. inversion H1.
-  simpl. unfold gempty. reflexivity.
-
-  destruct (ge a) eqn:?.
-  Focus 2.
-  assert (In a (a :: x)) by (simpl; left; reflexivity).
-  erewrite <- H in H1. congruence.
-
-  remember (fun id => if ident_eq id a then None else ge id) as ge'.
-  assert (forall id, ge' id <> None <-> In id x). {
-    admit. (* idents ignore second part, which is hard *)
-    (* this is not quite true both ways, backwards In id x -> ge' id <> None is hard *)
-  }
-
-  eapply IHx in H1.
-  destruct H1 as [l'].
-  exists ((a,e) :: l').
-  intros.
-  simpl. unfold extend.
-  unfold name_irrel in H0.
-  specialize (H0 id a).
-  destruct (ident_eq id a) eqn:?.
-  congruence.
-  rewrite <- H1.
-  subst ge'.
-  rewrite Heqs. reflexivity.
-  subst ge'.
-  eapply name_irrel_erase; eauto.
-Admitted.
-*)
-
-
-(*  intros. eapply global_extends_eager_eval'; eauto.
-Qed.*)
-
-(* Add a list to the GE that is all the things that GE contains *)
-(*
-Lemma eager_eval_expr_ident_irrel :
-  forall ge id,
-    ge id = None ->
-    (forall id' exp',
-        ge id' = Some exp' ->
-        forall id0 exp0 TE SE v,
-          eager_eval_expr ge TE SE exp' v ->
-          eager_eval_expr (extend ge id0 exp0) TE SE exp' v) ->
-    name_irrel ge ->
-    forall expr TE SE v,
-      eager_eval_expr ge TE SE expr v ->
-      forall v',
-        eager_eval_expr (extend ge id v') TE SE expr v.
-Proof. 
-  intros ge id Hnon Hnirr expr.
-  eapply Expr_ind_useful with (e := expr); intros.
-  * inversion H0. subst.
-    econstructor; eauto.
-    admit. admit.
-
-  * inversion H0. subst.
-    econstructor; eauto.
-    unfold Pl in H.
-    eapply Forall_Forall2_implies; try eapply H2; try eapply H.
-    intros. eauto.
-
-  * admit.
-
-  * admit.
-
-  * admit.
-  * admit.
-  * admit.
-  * inversion H.
-    subst. econstructor; eauto.
-    subst.
-    edestruct (@name_irrel_diff_results Expr); try eassumption; try congruence.
-    instantiate (1 := id). instantiate (1 := id0).
-    congruence.
-    eapply eager_eval_global_var. eauto.
-    unfold extend. rewrite H0.
-    eauto.
-    
-    
-Admitted.
-
-Lemma eager_eval_expr_ident_irrel_parallel :
-  forall expr ge ge' TE SE v,
-    (eager_eval_expr ge TE SE expr v -> 
-    eager_eval_expr ge' TE SE expr v) ->
-    forall id exp,
-      eager_eval_expr (extend ge id exp) TE SE expr v ->
-      eager_eval_expr (extend ge' id exp) TE SE expr v.
-Proof.
-Admitted.
- *)
-
-(*  intros.
-  unfold global_extends in *.
-  destruct H. split.
-  intros.
-  unfold extend.
-  remember H3 as Hsome.
-  clear HeqHsome.
-  eapply H in H3.
-  rewrite H3.
-  destruct (ident_eq id0 id) eqn:?; auto.
-  unfold name_irrel in *.
-  specialize (H0 id0 id).
-  rewrite Heqs in H0. congruence.
-
-  intros.
-  eapply eager_eval_expr_ident_irrel in H1; eauto.
-  eapply H2 in H3.
-  eapply eager_eval_expr_ident_irrel_parallel.
-  eapply H2. eauto.
-Qed.
-*)
